Merge branch 'master' of ssh://github.mit.edu/plv/fiat

src/Common/List/Prefix.v
@@ -5,29 +5,28 @@ Section Prefix.
   Context {A : Type}.
   Context {A_eq_dec : forall (a a' : A), {a = a'} + {a <> a'}}.
 
-  Definition prefixProp (p s : list A) := exists ps, p ++ ps = s.
+  Definition prefix_prop (p s : list A) := exists ps, p ++ ps = s.
 
-  Fixpoint prefixBool (p s : list A) :=
+  Fixpoint prefix_bool (p s : list A) :=
     match p, s with
-      | nil , _ => true
-      | p' :: ps', s' :: ss' => if A_eq_dec p' s' then prefixBool ps' ss' else false
+      | nil, _ => true
+      | p' :: ps', s' :: ss' => if A_eq_dec p' s' then prefix_bool ps' ss' else false
       | _, _ => false
     end.
 
-  Lemma prefixBool_eq :
-    forall (p s : list A),
-      prefixBool p s = true <-> prefixProp p s.
+  Lemma prefix_bool_eq :
+    forall (p s : list A), prefix_bool p s = true <-> prefix_prop p s.
   Proof.
-    unfold prefixProp; split; revert s; induction p; intros s H.
-    - eexists s; reflexivity.
-    - destruct s; simpl in H.
-      + discriminate.
-      + find_if_inside; [subst | discriminate].
-        apply_in_hyp IHp; destruct_ex; eexists; subst; reflexivity.
-    - simpl; reflexivity.
-    - destruct s; simpl in *; destruct H.
-      + discriminate.
-      + injections; find_if_inside; intuition eauto.
+    unfold prefix_prop, prefix_bool; split; revert s; induction p; intros s H; [
+      eexists s; reflexivity |
+      destruct s; simpl in H; [
+        discriminate |
+        find_if_inside; [subst | discriminate];
+        apply_in_hyp IHp; destruct_ex; eexists; subst; reflexivity ] |
+      reflexivity |
+      destruct s; simpl in *; destruct H; [
+        discriminate |
+        injections; find_if_inside; intuition eauto ] ].
   Qed.
 
 End Prefix.
