src/Parsers/BooleanRecognizerCorrect.v
@@ -1,5 +1,6 @@
 (** * Definition of a boolean-returning CFG parser-recognizer *)
 Require Import Coq.Lists.List Coq.Program.Program Coq.Program.Wf Coq.Arith.Wf_nat Coq.Arith.Compare_dec Coq.Classes.RelationClasses Coq.Strings.String.
+Require Import Coq.omega.Omega.
 Require Import ADTSynthesis.Parsers.ContextFreeGrammar ADTSynthesis.Parsers.BooleanRecognizer ADTSynthesis.Parsers.MinimalParse.
 Require Import ADTSynthesis.Parsers.BaseTypes ADTSynthesis.Parsers.BooleanBaseTypes.
 Require Import ADTSynthesis.Parsers.Splitters.RDPList ADTSynthesis.Parsers.Splitters.BruteForce.
